unique_ids2.thy
@@ -14,153 +14,293 @@ begin
 
 definition 
   "new_unique_not_in_invocationOp iop uidv \<equiv>
-\<forall>i op. iop i \<triangleq> op \<longrightarrow> to_nat uidv \<notin> uniqueIds op "
+\<forall>i op. iop i \<triangleq> op \<longrightarrow> uidv \<notin> uniqueIds op "
 
 
 definition 
   "new_unique_not_in_calls iop uidv \<equiv>
-\<forall>i op r. iop i \<triangleq> Call op r \<longrightarrow> to_nat uidv \<notin> uniqueIds op "
+\<forall>i op r. iop i \<triangleq> Call op r \<longrightarrow> uidv \<notin> uniqueIds op "
 
 definition 
   "new_unique_not_in_calls_result iop uidv \<equiv>
-\<forall>i op r. iop i \<triangleq> Call op r \<longrightarrow> to_nat uidv \<notin> uniqueIds r "
+\<forall>i op r. iop i \<triangleq> Call op r \<longrightarrow> uidv \<notin> uniqueIds r "
 
 definition
 "new_unique_not_in_invocationRes ires uidv \<equiv> 
-\<forall>i r. ires i \<triangleq> r \<longrightarrow> to_nat uidv \<notin> uniqueIds r "
+\<forall>i r. ires i \<triangleq> r \<longrightarrow> uidv \<notin> uniqueIds r "
+
+definition
+"new_unique_not_in_other_invocations i los p uidv \<equiv>
+(\<forall>i' ls impl. i' \<noteq> i \<longrightarrow> los i' \<triangleq> ls \<longrightarrow> p i' \<triangleq> impl \<longrightarrow> (\<exists>uids. uidv \<notin> uids \<and> procedure_cannot_guess_ids uids ls impl))"
 
 
-(* TODO hmm, I have the feeling that I already did something similar ... *)
+lemma show_new_unique_not_in_other_invocations:
+  assumes a1: "new_unique_not_in_other_invocations i los p uidv"
+    and a2: "\<And>i' uids ls ls' impl. \<lbrakk>i' \<noteq> i; los i' \<triangleq> ls; los' i' \<triangleq> ls'; p i' \<triangleq> impl;  procedure_cannot_guess_ids uids ls impl\<rbrakk> \<Longrightarrow> procedure_cannot_guess_ids uids ls' impl"
+    and a3: "dom los = dom los'"
+  shows "new_unique_not_in_other_invocations i los' p uidv"
+proof (auto simp add: new_unique_not_in_other_invocations_def)
+  fix i' ls impl
+  assume b1: "i' \<noteq> i"
+    and b2: "los' i' \<triangleq> ls"
+    and b3: "p i' \<triangleq> impl"
+
+  obtain ls_pre where b4: "los i' \<triangleq> ls_pre"
+    using a3 b2 by force
+
+
+  from a1 obtain uids where b5: " uidv \<notin> uids" and b6: "procedure_cannot_guess_ids uids ls_pre impl"
+    by (meson b1 b3 b4 new_unique_not_in_other_invocations_def)
+
+  have "procedure_cannot_guess_ids uids ls impl"
+    using b1 b4 b2 b3 b6 by (rule a2)
+
+  show "\<exists>uids.  uidv \<notin> uids \<and> procedure_cannot_guess_ids uids ls impl"
+    using \<open>procedure_cannot_guess_ids uids ls impl\<close> b5 by auto
+qed
+
+definition uid_is_private where
+"uid_is_private i s_calls s_invocationOp s_invocationRes s_knownIds s_generatedIds s_localState s_currentProc uidv  \<equiv> 
+new_unique_not_in_invocationOp s_invocationOp uidv
+    \<and> new_unique_not_in_calls s_calls uidv
+    \<and> new_unique_not_in_calls_result s_calls uidv
+    \<and> new_unique_not_in_invocationRes s_invocationRes uidv
+    \<and> uidv \<notin> s_knownIds
+    \<and> s_generatedIds uidv \<triangleq> i
+    \<and> new_unique_not_in_other_invocations i s_localState s_currentProc uidv"
+
+
+lemma growth_still_hidden_step_other:
+  assumes S_wf: "state_wellFormed S"
+    and prog_wf: "program_wellFormed (prog S)"
+    and p1: "uid_is_private i (calls S) (invocationOp S) (invocationRes S) (knownIds S) (generatedIds S) (localState S) (currentProc S) uidv"
+    and step: "S ~~ (i', a) \<leadsto> S'"
+    and other: "i' \<noteq> i"
+  shows "uid_is_private i (calls S') (invocationOp S') (invocationRes S') (knownIds S') (generatedIds S') (localState S') (currentProc S') uidv"
+proof -
+
+
+  have priv_S: "uid_is_private i (calls S) (invocationOp S) (invocationRes S) (knownIds S) (generatedIds S) (localState S)
+         (currentProc S) uidv"
+    by (simp add: p1)
+
+
+  have i1: "new_unique_not_in_invocationOp (invocationOp S) uidv "
+    by (meson priv_S uid_is_private_def)
+
+
+  have i2: "new_unique_not_in_calls (calls S) uidv "
+    by (meson priv_S uid_is_private_def)
+  have i3: "new_unique_not_in_calls_result (calls S) uidv"
+    by (meson priv_S uid_is_private_def)
+  have i4: "new_unique_not_in_invocationRes (invocationRes S) uidv"
+    by (meson priv_S uid_is_private_def)
+  have i5: "uidv \<notin> knownIds S"
+    by (meson priv_S uid_is_private_def)
+  have i6: "new_unique_not_in_other_invocations i (localState S) (currentProc S) uidv"
+    by (meson priv_S uid_is_private_def)
+
+  have still_generated: "generatedIds S uidv \<triangleq> i"
+    by (meson priv_S uid_is_private_def)
+
+
+  note invs = i1 i2 i3 i4 i5 i6 still_generated
+
+
+
+  have i6': "\<And>ls impl. localState S i' \<triangleq> ls \<Longrightarrow> currentProc S i' \<triangleq> impl \<Longrightarrow> (\<exists>uids.  uidv \<notin> uids \<and> procedure_cannot_guess_ids uids ls impl)"
+    using \<open>i' \<noteq> i\<close> i6
+    by (meson new_unique_not_in_other_invocations_def) 
+
+
+
+  have S'_wf: "state_wellFormed S'" if noFail: "a \<noteq> AFail"
+    using S_wf local.step noFail state_wellFormed_combine1 by blast
+
+
+
+
+  from `S ~~ (i', a) \<leadsto> S'`
+  show ?thesis
+  proof (induct rule: step.cases)
+    case (local S i2 ls f ls')
+
+    obtain uids where  uids1: " uidv \<notin> uids" and uids2: "procedure_cannot_guess_ids uids ls f"
+      using \<open>i' \<noteq> i\<close> i6 local i6' by auto 
+
+    from local
+    show ?case
+      using invs  apply (auto simp add: uid_is_private_def elim!: show_new_unique_not_in_other_invocations split: if_splits)
+      by (meson pcgi_local_case uids1 uids2)
+
+
+
+  next
+    case (newId S i' ls f ls' uid uidv ls'')
+    show ?case 
+      using invs  apply (auto simp add: uid_is_private_def newId)
+      using `uid = to_nat uidv` `generatedIds S uid = None` apply auto[1]
+      using `uid = to_nat uidv` `generatedIds S uid = None`  apply (auto simp add: new_unique_not_in_other_invocations_def)
+      by (metis (no_types, lifting) Un_insert_right insert_iff newId.hyps(4) newId.hyps(5) newId.hyps(6) newId.hyps(8) newId.hyps(9) option.inject pcgi_newId_case sup_bot.comm_neutral)
+
+
+  next
+    case (beginAtomic S i ls f ls' t vis snapshot)
+    then show ?case using invs by (auto simp add: uid_is_private_def pcgi_beginAtomic_case elim!: show_new_unique_not_in_other_invocations split: if_splits)
+  next
+    case (endAtomic S i ls f ls' t)
+    then show ?case using invs 
+      by (auto simp add: uid_is_private_def pcgi_endAtomic_case elim!: show_new_unique_not_in_other_invocations split: if_splits)
+
+
+
+
+  next
+    case (dbop S i' ls f Op ls' t c res vis)
+
+    obtain uids where  uids1: " uidv \<notin> uids" and uids2: "procedure_cannot_guess_ids uids ls f"
+      using dbop.hyps(1) dbop.hyps(2) dbop.hyps(4) dbop.hyps(5) i6' by blast 
+
+
+
+    from pcgi_dbop_case1[OF uids2 `f ls = DbOperation Op ls'`]
+    have "uniqueIds Op \<subseteq> uids" .
+
+    with uids1 have uids2: " uidv \<notin> uniqueIds Op"
+      by auto
+
+    have qcngi: "queries_cannot_guess_ids (querySpec (prog S))"
+      using dbop.hyps(1) prog_wf program_wellFormed_def by blast
+
+
+
+    have uids3: " uidv \<notin> uniqueIds res"
+    proof (rule notI)
+      assume " uidv \<in> uniqueIds res "
+
+      from qcngi `querySpec (prog S) Op (getContext S i') res` ` uidv \<in> uniqueIds res` ` uidv \<notin> uniqueIds Op`
+      have "\<exists>cId opr res. calls (getContext S i') cId \<triangleq> Call opr res \<and>  uidv \<in> uniqueIds opr"
+        by (rule queries_cannot_guess_ids_def2[THEN iffD1, rule_format])
+
+      thus False
+        apply (auto simp add: getContextH_def restrict_map_def split: option.splits if_splits)
+        using dbop.hyps(1) i2 new_unique_not_in_calls_def by fastforce
+    qed
+
+
+
+
+    show ?case 
+    proof (auto simp add: uid_is_private_def dbop invs uids2 uids3 )
+      show "new_unique_not_in_invocationOp (invocationOp S) uidv"
+        using dbop.hyps(1) i1 by blast
+
+
+      show "new_unique_not_in_calls (calls S(c \<mapsto> Call Op res)) uidv"
+        using uids2 i2 by (auto simp add: new_unique_not_in_calls_def dbop )
+
+      show " new_unique_not_in_calls_result (calls S(c \<mapsto> Call Op res)) uidv"
+        using uids2 i3 by (auto simp add: new_unique_not_in_calls_result_def dbop uids3)
+
+
+      show "new_unique_not_in_invocationRes (invocationRes S) uidv"
+        using dbop.hyps(1) i4 by blast
+
+      show " uidv \<in> knownIds S \<Longrightarrow> False"
+        using dbop.hyps(1) i5 by blast
+
+      show "new_unique_not_in_other_invocations i (localState S(i' \<mapsto> ls' res)) (currentProc S) uidv"
+        by (smt UnE \<open>\<And>thesis. (\<And>uids. \<lbrakk>uidv \<notin> uids; procedure_cannot_guess_ids uids ls f\<rbrakk> \<Longrightarrow> thesis) \<Longrightarrow> thesis\<close> dbop.hyps(1) dbop.hyps(5) dbop.hyps(6) fun_upd_other fun_upd_same i6 new_unique_not_in_other_invocations_def option.sel pcgi_dbop_case2 uids3)
+
+
+      show "generatedIds S uidv \<triangleq> i"
+        using dbop.hyps(1) still_generated by blast
+
+    qed
+
+
+
+
+
+  next
+    case (invocation S i proc initialState impl)
+    then show ?case using invs apply (auto simp add: uid_is_private_def)
+       apply (auto simp add: new_unique_not_in_invocationOp_def)
+      apply (auto simp add: new_unique_not_in_other_invocations_def)
+      by (metis prog_wf program_wellFormed_def show_procedures_cannot_guess_ids subsetD subset_Un_eq subset_refl)
+
+  next
+    case (return S i ls f res)
+    then show ?case using invs apply (auto simp add: uid_is_private_def)
+        apply (auto simp add: new_unique_not_in_invocationRes_def)
+      using i6' pcgi_return_case apply fastforce
+      using i6' pcgi_return_case apply fastforce
+      by (simp add: new_unique_not_in_other_invocations_def)
+
+  next
+    case (fail S i ls)
+    then show ?case 
+      using invs
+      by (auto simp add: uid_is_private_def new_unique_not_in_other_invocations_def)
+
+
+  next
+    case (invCheck S res i)
+    then show ?case using invs by (auto simp add: uid_is_private_def)
+  qed
+qed
+
+
+lemma growth_still_hidden_steps_other:
+  assumes S_wf: "state_wellFormed S"
+    and prog_wf: "program_wellFormed (prog S)"
+    and p1: "uid_is_private i (calls S) (invocationOp S) (invocationRes S) (knownIds S) (generatedIds S) (localState S) (currentProc S) uidv"
+    and steps: "S ~~ tr \<leadsto>* S'"
+    and other: "\<forall>(i',a)\<in>set tr. i' \<noteq> i"
+    and no_fail: "\<forall>i. (i, AFail) \<notin> set tr"
+  shows "uid_is_private i (calls S') (invocationOp S') (invocationRes S') (knownIds S') (generatedIds S') (localState S') (currentProc S') uidv"
+using steps   p1 other no_fail proof (induct rule: steps_induct)
+  case initial
+  then show ?case by simp
+next
+  case (step S' tr a S'')
+  
+  show ?case 
+    using  `S' ~~ a \<leadsto> S''`
+  proof (fuzzy_rule growth_still_hidden_step_other)
+    show "state_wellFormed S'"
+      using S_wf state_wellFormed_combine step.prems step.steps by fastforce
+
+    show "a = (fst a, snd a)" by force
+    show "fst a \<noteq> i"
+      using local.step by auto
+    show "program_wellFormed (prog S')"
+      using prog_wf step.steps steps_do_not_change_prog by fastforce
+    show "uid_is_private i (calls S') (invocationOp S') (invocationRes S') (knownIds S') (generatedIds S') (localState S')
+     (currentProc S') uidv"
+      using step by auto
+  qed
+qed
+
+
+
 lemma growth_still_hidden:
   assumes g: "state_monotonicGrowth i S S'"
     and prog_wf: "program_wellFormed (prog S)"
-    and a1: "new_unique_not_in_invocationOp (invocationOp S) uidv"
-    and a2: "new_unique_not_in_calls (calls S) uidv"
-    and a3: "new_unique_not_in_calls_result (calls S) uidv"
-    and a4: "new_unique_not_in_invocationRes (invocationRes S) uidv"
-    and a5: "to_nat uidv \<notin> knownIds S"
-    and a6: "generatedIds S (to_nat uidv) \<triangleq> i"
-shows "new_unique_not_in_invocationOp (invocationOp S') uidv
-\<and> new_unique_not_in_calls (calls S') uidv
-\<and> new_unique_not_in_calls_result (calls S') uidv
-\<and> new_unique_not_in_invocationRes (invocationRes S') uidv
-\<and> to_nat uidv \<notin> knownIds S'"
+    and p1: "uid_is_private i (calls S) (invocationOp S) (invocationRes S) (knownIds S) (generatedIds S) (localState S) (currentProc S) uidv"
+  shows "uid_is_private i (calls S') (invocationOp S') (invocationRes S') (knownIds S') (generatedIds S') (localState S') (currentProc S') uidv"
 proof -
   from g obtain tr
     where wf: "state_wellFormed S"
-    and steps: "S ~~ tr \<leadsto>* S'"
-    and no_i: "\<forall>x\<in>set tr. case x of (i', a) \<Rightarrow> i' \<noteq> i"
-    and no_fail: "\<forall>i. (i, AFail) \<notin> set tr"
+      and steps: "S ~~ tr \<leadsto>* S'"
+      and no_i: "\<forall>x\<in>set tr. case x of (i', a) \<Rightarrow> i' \<noteq> i"
+      and no_fail: "\<forall>i. (i, AFail) \<notin> set tr"
     by (auto simp add: state_monotonicGrowth_def)
 
 
-  from steps no_i wf no_fail prog_wf a1 a2 a3 a4 a5 a6
+  from steps no_i wf no_fail prog_wf p1
   show ?thesis
-  proof (induct rule: steps.induct)
-    case (steps_refl S)
-    then show ?case
-      by auto
-  next
-    case (steps_step S1 tr S2 a S3)
-
-
-    have "new_unique_not_in_invocationOp (invocationOp S2) uidv \<and>
-        new_unique_not_in_calls (calls S2) uidv \<and>
-        new_unique_not_in_calls_result (calls S2) uidv \<and>
-        new_unique_not_in_invocationRes (invocationRes S2) uidv \<and> to_nat uidv \<notin> knownIds S2"
-      by (rule steps_step, insert `\<forall>i. (i, AFail) \<notin> set (tr @ [a])`,auto simp add: steps_step)
-
-    hence i1: "new_unique_not_in_invocationOp (invocationOp S2) uidv "
-      and i2: "new_unique_not_in_calls (calls S2) uidv "
-      and i3: "new_unique_not_in_calls_result (calls S2) uidv"
-      and i4: "new_unique_not_in_invocationRes (invocationRes S2) uidv"
-      and i5: "to_nat uidv \<notin> knownIds S2"
-      by (auto simp add: steps_step)
-
-    note invs = i1 i2 i3 i4 i5
-   
-
-    from `S2 ~~ a \<leadsto> S3`
-    show ?case
-    proof (induct rule: step.cases)
-      case (local S i ls f ls')
-      then show ?case
-        using invs by (auto simp add: )
-    next
-      case (newId S i ls f ls' uid uidv ls'')
-      then show ?case 
-        using invs by (auto simp add: )
-    next
-      case (beginAtomic S i ls f ls' t vis snapshot)
-      then show ?case using invs by (auto simp add: )
-    next
-      case (endAtomic S i ls f ls' t)
-      then show ?case using invs by (auto simp add: )
-    next
-      case (dbop S i ls f Op ls' t c res vis)
-      from dbop 
-      show ?case using invs 
-      proof (auto simp add: )
-
-        show "new_unique_not_in_calls (\<lambda>a. if a = c then Some (Call Op res) else calls S a) uidv"
-          if c0: "S2 = S"
-            and c1: "a = (i, ADbOp c Op res)"
-            and c2: "S3 = S \<lparr>localState := localState S(i \<mapsto> ls' res), calls := calls S(c \<mapsto> Call Op res), callOrigin := callOrigin S(c \<mapsto> t), visibleCalls := visibleCalls S(i \<mapsto> insert c vis), happensBefore := happensBefore S \<union> vis \<times> {c}\<rparr>"
-            and c3: "localState S i \<triangleq> ls"
-            and c4: "currentProc S i \<triangleq> f"
-            and c5: "f ls = DbOperation Op ls'"
-            and c6: "currentTransaction S i \<triangleq> t"
-            and c7: "calls S c = None"
-            and c8: "querySpec (prog S) Op (getContextH (calls S) (happensBefore S) (Some vis)) res"
-            and c9: "visibleCalls S i \<triangleq> vis"
-            and c10: "new_unique_not_in_invocationOp (invocationOp S) uidv"
-            and c11: "new_unique_not_in_calls (calls S) uidv"
-            and c12: "new_unique_not_in_calls_result (calls S) uidv"
-            and c13: "new_unique_not_in_invocationRes (invocationRes S) uidv"
-            and c14: "to_nat uidv \<notin> knownIds S"
-          sorry
-
-        show "new_unique_not_in_calls_result (\<lambda>a. if a = c then Some (Call Op res) else calls S a) uidv"
-          if c0: "S2 = S"
-            and c1: "a = (i, ADbOp c Op res)"
-            and c2: "S3 = S \<lparr>localState := localState S(i \<mapsto> ls' res), calls := calls S(c \<mapsto> Call Op res), callOrigin := callOrigin S(c \<mapsto> t), visibleCalls := visibleCalls S(i \<mapsto> insert c vis), happensBefore := happensBefore S \<union> vis \<times> {c}\<rparr>"
-            and c3: "localState S i \<triangleq> ls"
-            and c4: "currentProc S i \<triangleq> f"
-            and c5: "f ls = DbOperation Op ls'"
-            and c6: "currentTransaction S i \<triangleq> t"
-            and c7: "calls S c = None"
-            and c8: "querySpec (prog S) Op (getContextH (calls S) (happensBefore S) (Some vis)) res"
-            and c9: "visibleCalls S i \<triangleq> vis"
-            and c10: "new_unique_not_in_invocationOp (invocationOp S) uidv"
-            and c11: "new_unique_not_in_calls (calls S) uidv"
-            and c12: "new_unique_not_in_calls_result (calls S) uidv"
-            and c13: "new_unique_not_in_invocationRes (invocationRes S) uidv"
-            and c14: "to_nat uidv \<notin> knownIds S"
-          sorry
-      qed
-
-
-
-
-
-    next
-      case (invocation S i proc initialState impl)
-      then show ?case using invs apply (auto simp add: )
-        by (auto simp add: new_unique_not_in_invocationOp_def)
-    next
-      case (return S i ls f res)
-      then show ?case using invs apply (auto simp add: )
-         apply (auto simp add: new_unique_not_in_invocationRes_def)
-        sorry
-
-    next
-      case (fail S i ls)
-      then show ?case using invs by (auto simp add: )
-    next
-      case (invCheck S res i)
-      then show ?case using invs by (auto simp add: )
-    qed
-  qed
+    using growth_still_hidden_steps_other by blast
 qed
 
 
